x86/LocalLib.v
@@ -9,9 +9,13 @@ Require Import Globalenvs.
 Import ListNotations.
 
 
-Axiom unsigned_repr: forall n, Ptrofs.unsigned (Ptrofs.repr n) = n.
 
 Definition alignw:Z := 8.
+
+Lemma alignw0: (alignw | 0).
+Proof.
+  red. exists 0. omega.
+Qed.
 
 Ltac destr_if := 
   match goal with 
@@ -1034,7 +1038,9 @@ Proof.
   erewrite <- Genv.store_zeros_perm; eauto.
 Qed.
 
-Lemma store_zeros_extend: forall m1 m1' b lo hi lo' hi' m2,
+Axiom unsigned_repr: forall n, Ptrofs.unsigned (Ptrofs.repr n) = n.
+
+Axiom store_zeros_extend: forall m1 m1' b lo hi lo' hi' m2,
     Mem.extends m1 m1' ->
     store_zeros m1 b lo hi = Some m2 ->
     lo' <= lo ->
@@ -1042,17 +1048,13 @@ Lemma store_zeros_extend: forall m1 m1' b lo hi lo' hi' m2,
     (forall ofs k p, lo' <= ofs < lo \/ hi <= ofs < hi' -> ~ Mem.perm m1 b ofs k p) ->
     exists m2', store_zeros m1' b lo' hi' = Some m2' /\
            Mem.extends m2 m2'.
-Proof.
-Admitted.  
 
-Lemma store_init_data_list_extends: forall {F V} (ge tge: Genv.t F V) l1 l2 m1 m1' m2 b ofs,
+Axiom store_init_data_list_extends: forall {F V} (ge tge: Genv.t F V) l1 l2 m1 m1' m2 b ofs,
     (forall b, Genv.find_symbol ge b = Genv.find_symbol tge b) ->
     Mem.extends m1 m1' ->
     Genv.store_init_data_list ge m1 b ofs l1 = Some m2 ->
     exists m2', Genv.store_init_data_list tge m1' b ofs (l1 ++ l2) = Some m2' /\
            Mem.extends m2 m2'.
-Admitted.
-
 
 Lemma init_data_alignment_pos: forall id,
     0 < Genv.init_data_alignment id.
